Isabelle2/AbstractMultiPaxosR1Correctness.thy
@@ -72,29 +72,29 @@ lemma inv2: "invariant the_ioa inv2"  by (try_inv invs:inv1)
 
 definition inv3 where inv3_def[inv_defs]:
   -- {* acceptors only vote for the suggestion. *}
-  "inv3 s \<equiv> \<forall> i a b . let v = vote s i a b in v \<noteq> None \<longrightarrow> v = suggestion s i b"
+  "inv3 s \<equiv> \<forall> i a b . let v = vote s a i b in v \<noteq> None \<longrightarrow> v = suggestion s i b"
 
 lemma inv3: "invariant the_ioa inv3"  by (try_inv invs:inv1 inv2)
 
-abbreviation conservative_array where
-  "conservative_array s \<equiv>  \<forall> i . ballot_array.conservative_array (vote s i)"
+definition conservative where
+  "conservative s \<equiv>  \<forall> i . ballot_array.conservative_array (flip (vote s) i)"
 
-lemma conservative: "invariant the_ioa conservative_array"
+lemma conservative: "invariant the_ioa conservative"
 proof -
-  have "\<And> s . inv3 s \<Longrightarrow> conservative_array s"
+  have "\<And> s . inv3 s \<Longrightarrow> conservative s"
     apply (simp add:inv_defs ballot_array.conservative_def ballot_array.conservative_array_def
-        split:option.splits) by (metis option.inject) 
+       conservative_def split:option.splits) by (metis option.inject)
   with inv3 show ?thesis  using IOA.invariant_def by blast
 qed
 
-abbreviation safe_at where "safe_at s i \<equiv> ballot_array.safe_at quorums (ballot s) (vote s i)"
+abbreviation safe_at where "safe_at s i \<equiv> ballot_array.safe_at quorums (ballot s) (flip (vote s) i)"
 
 lemma safe_mono:
   -- {* @{term safe_at} is monotonic. A key lemma to simplify invariant proofs. *}
   assumes "s \<midarrow>a\<midarrow>the_ioa\<longrightarrow> t" and "safe_at s i v b"
   shows "safe_at t i v b"
 proof -
-  have "is_prefix (ballot s) (ballot t) (vote s i) (vote t i)" using \<open>s \<midarrow>a\<midarrow>the_ioa\<longrightarrow> t\<close>
+  have "is_prefix (ballot s) (ballot t) (flip (vote s) i) (flip (vote t) i)" using \<open>s \<midarrow>a\<midarrow>the_ioa\<longrightarrow> t\<close>
     by (simp add:inv_defs ioa_defs; induct_tac rule:trans_cases, auto simp add:is_prefix_def inv_defs split:option.split_asm)
   thus ?thesis
   using assms ballot_array_prefix.safe_at_mono
@@ -105,8 +105,8 @@ context begin
 
 definition inv4 where inv4_def[inv_defs]:
   "inv4 s \<equiv> \<forall> b i q . joined s q b \<and> q \<in> quorums \<longrightarrow> 
-  (case sugg s i b q of  Some v \<Rightarrow> dsa.proved_safe_at (ballot s) (vote s i) q b v
-  | None \<Rightarrow> (\<forall> v . dsa.proved_safe_at (ballot s) (vote s i) q b v))"
+  (case sugg s i b q of  Some v \<Rightarrow> dsa.proved_safe_at (ballot s) (flip (vote s) i) q b v
+  | None \<Rightarrow> (\<forall> v . dsa.proved_safe_at (ballot s) (flip (vote s) i) q b v))"
   
 text {* To show that @{term inv4} is invariant, we will use two auxiliary invariants. *}
 
@@ -114,12 +114,12 @@ text {* First, we show that an acceptor that has sent a oneb for ballot b has in
   its maximum vote before b. *}
 
 definition inv4_1 where "inv4_1 s \<equiv> \<forall> a b f i . onebs s a b = Some f 
-      \<longrightarrow> f i = dsa.acc_max (vote s i) a b \<and> ballot s a \<ge> b"
+      \<longrightarrow> f i = dsa.acc_max (flip (vote s) i) a b \<and> ballot s a \<ge> b"
 
 text {* Then, we show that @{term max_vote} is the maximum vote before b over a quorum that has joined b. *}
 
 definition inv4_2 where "inv4_2 s \<equiv> \<forall> i b q . joined s q b \<longrightarrow> 
-    (max_vote s i b q = dsa.max_quorum_votes (vote s i) q b) \<and> (\<forall> a \<in> q . ballot s a \<ge> b)"
+    (max_vote s i b q = dsa.max_quorum_votes (flip (vote s) i) q b) \<and> (\<forall> a \<in> q . ballot s a \<ge> b)"
   
 private 
 lemma inv4_1:"invariant the_ioa inv4_1"
@@ -131,15 +131,15 @@ lemma inv4_1:"invariant the_ioa inv4_1"
     fix a b f i
     assume "onebs t a b = Some f"
     hence "onebs s a b = Some f" using \<open>do_vote a2 i2 v s t\<close> unfolding do_vote_def by auto
-    hence "f i = dsa.acc_max (vote s i) a b" and "b \<le> ballot s a" using \<open>inv4_1 s\<close> unfolding inv4_1_def by auto
-    have "dsa.acc_max (vote t i) a b = dsa.acc_max (vote s i) a b"
+    hence "f i = dsa.acc_max (flip (vote s) i) a b" and "b \<le> ballot s a" using \<open>inv4_1 s\<close> unfolding inv4_1_def by auto
+    have "dsa.acc_max (flip (vote t) i) a b = dsa.acc_max (flip (vote s) i) a b"
     proof -
-      from \<open>b \<le> ballot s a\<close> have "\<And> b' . b' < b \<Longrightarrow> vote s i a b' = vote t i a b'" using  \<open>do_vote a2 i2 v s t\<close>
+      from \<open>b \<le> ballot s a\<close> have "\<And> b' . b' < b \<Longrightarrow> flip (vote s) i a b' = flip (vote t) i a b'" using  \<open>do_vote a2 i2 v s t\<close>
         unfolding do_vote_def by auto
-      hence "{(v, ba). ba < b \<and> vote s i a ba = Some v} = {(v, ba). ba < b \<and> vote t i a ba = Some v}" by metis
+      hence "{(v, ba). ba < b \<and> flip (vote s) i a ba = Some v} = {(v, ba). ba < b \<and> flip (vote t) i a ba = Some v}" by metis
       thus ?thesis unfolding dsa.acc_max_def dsa.a_votes_def by auto
     qed
-    with \<open>f i = dsa.acc_max (vote s i) a b\<close> show "f i = dsa.acc_max (vote t i) a b" by auto
+    with \<open>f i = dsa.acc_max (flip (vote s) i) a b\<close> show "f i = dsa.acc_max (flip (vote t) i) a b" by auto
     from \<open>b \<le> ballot s a\<close> and \<open>do_vote a2 i2 v s t\<close> show "b \<le> ballot t a" unfolding do_vote_def by auto
   qed
   done
@@ -151,9 +151,9 @@ proof -
   proof (clarsimp, rule conjI)
     fix i b q
     assume "joined s q b"
-    hence "(the (onebs s a b)) i = dsa.acc_max (vote s i) a b" if "a \<in> q" for a
+    hence "(the (onebs s a b)) i = dsa.acc_max (flip (vote s) i) a b" if "a \<in> q" for a
       using \<open>inv4_1 s\<close> that by (simp add: ampr1_ioa.joined_def inv4_1_def) 
-    thus "max_vote s i b q = dsa.max_quorum_votes (vote s i) q b" 
+    thus "max_vote s i b q = dsa.max_quorum_votes (flip (vote s) i) q b" 
       unfolding max_vote_def dsa.max_quorum_votes_def by auto
     show "\<forall>a\<in>q. b \<le> ballot s a" using \<open>inv4_1 s\<close> \<open>joined s q b\<close> unfolding joined_def inv4_1_def by auto
   qed
@@ -162,72 +162,72 @@ qed
 
 lemma inv4:"invariant the_ioa inv4"
 proof -
-  have "inv4 s" if "inv4_2 s" and "conservative_array s" for s unfolding inv4_def
+  have "inv4 s" if "inv4_2 s" and "conservative s" for s unfolding inv4_def
   proof (clarify)
     fix b i q
     assume  "joined s q b" and "q \<in> quorums"
-    have "max_vote s i b q = dsa.max_quorum_votes (vote s i) q b" by (metis \<open>joined s q b\<close>  \<open>inv4_2 s\<close> inv4_2_def)
-    let ?proved="dsa.proved_safe_at (ballot s) (vote s i) q b"
+    have "max_vote s i b q = dsa.max_quorum_votes (flip (vote s) i) q b" by (metis \<open>joined s q b\<close>  \<open>inv4_2 s\<close> inv4_2_def)
+    let ?proved="dsa.proved_safe_at (ballot s) (flip (vote s) i) q b"
     show "case sugg s i b q of  Some v \<Rightarrow> ?proved v | None \<Rightarrow> (\<forall> v . ?proved v)"
     proof (cases "sugg s i b q")
       case None
-      hence "dsa.max_quorum_votes (vote s i) q b = {}" unfolding sugg_def
-          \<open>max_vote s i b q = dsa.max_quorum_votes (vote s i) q b\<close> by auto
+      hence "dsa.max_quorum_votes (flip (vote s) i) q b = {}" unfolding sugg_def
+          \<open>max_vote s i b q = dsa.max_quorum_votes (flip (vote s) i) q b\<close> by auto
       moreover from \<open>inv4_2 s\<close> and \<open>joined s q b\<close> have "\<And> a . a \<in> q \<Longrightarrow> ballot s a \<ge> b"
         using inv4_2_def by blast 
       ultimately show ?thesis using \<open>q \<in> quorums\<close> None unfolding dsa.proved_safe_at_def joined_def by auto 
     next
       case (Some v)
         -- {* Here the difficulty lies in the use of @{term the_elem} in @{thm sugg_def} *}
-      obtain x where "dsa.max_quorum_votes (vote s i) q b = {x}"
+      obtain x where "dsa.max_quorum_votes (flip (vote s) i) q b = {x}"
       proof -
         from Some have "max_vote s i b q \<noteq> {}" unfolding sugg_def by auto
         moreover
-        note \<open>max_vote s i b q = dsa.max_quorum_votes (vote s i) q b\<close>  and \<open>conservative_array s\<close> 
+        note \<open>max_vote s i b q = dsa.max_quorum_votes (flip (vote s) i) q b\<close>  and \<open>conservative s\<close> 
         moreover note dsa_p.max_vote_e_or_singleton
-        ultimately show ?thesis using that  by (metis \<open>q \<in> quorums\<close>) 
+        ultimately show ?thesis using that unfolding conservative_def by (metis \<open>q \<in> quorums\<close>) 
       qed
       moreover 
-      have "v = (the_elem (fst ` (dsa.max_quorum_votes (vote s i) q b)))" using Some \<open>joined s q b\<close> \<open>inv4_2 s\<close>
+      have "v = (the_elem (fst ` (dsa.max_quorum_votes (flip (vote s) i) q b)))" using Some \<open>joined s q b\<close> \<open>inv4_2 s\<close>
         by (auto simp add:inv4_2_def sugg_def)
       ultimately show ?thesis using \<open>q\<in>quorums\<close> \<open>joined s q b\<close> \<open>inv4_2 s\<close> Some
         unfolding dsa.proved_safe_at_def inv4_2_def by auto
     qed
   qed
-  thus ?thesis by (metis (mono_tags, lifting) IOA.invariant_def conservative inv4_2)
+  thus ?thesis using IOA.invariant_def conservative inv4_2 by blast 
 qed
 
 end
 
-abbreviation safe where "safe s \<equiv> \<forall> i . ballot_array.safe  quorums (ballot s) (vote s i)"
+abbreviation safe where "safe s \<equiv> \<forall> i . ballot_array.safe  quorums (ballot s) (flip (vote s) i)"
 declare ballot_array.safe_def[inv_defs]
 
 lemma aqcuire_leadership_safe:
   fixes a q s t i v safe_at 
-  defines "safe_at w \<equiv> dsa.safe_at (ballot t) (vote t i) w (ballot t a)"
-  assumes "acquire_leadership a q s t" and "inv4 s" and "safe s" and "conservative_array s"
+  defines "safe_at w \<equiv> dsa.safe_at (ballot t) (flip (vote t) i) w (ballot t a)"
+  assumes "acquire_leadership a q s t" and "inv4 s" and "safe s" and "conservative s"
   shows "case suggestion t i (ballot t a) of Some v \<Rightarrow> safe_at v | None \<Rightarrow> safe_at v"
     -- {* Using @{thm inv4} and @{thm dsa_p.proved_safe_at_imp_safe_at}, we show that chaging leader is safe. *}
 proof -
   let ?b = "ballot s a"
   have 1:"q \<in> quorums" and 2:"joined s q ?b" using \<open>inv4 s\<close> \<open>acquire_leadership a q s t\<close> by (auto simp add:inv4_def) 
-  hence 3:"case sugg s i ?b q of None \<Rightarrow> \<forall>v. dsa.proved_safe_at (ballot s) (vote s i) q ?b v 
-    | Some v \<Rightarrow> dsa.proved_safe_at (ballot s) (vote s i) q ?b v" using \<open>inv4 s\<close> using inv4_def by blast 
+  hence 3:"case sugg s i ?b q of None \<Rightarrow> \<forall>v. dsa.proved_safe_at (ballot s) (flip (vote s) i) q ?b v 
+    | Some v \<Rightarrow> dsa.proved_safe_at (ballot s) (flip (vote s) i) q ?b v" using \<open>inv4 s\<close> using inv4_def by blast 
   have 4:"vote s = vote t" and 5:"ballot s = ballot t"
     and 6:"suggestion t i ?b = sugg s i ?b q" using \<open>acquire_leadership a q s t\<close> by auto 
   show ?thesis
   proof (cases "suggestion t i ?b")
     case None
     with \<open>acquire_leadership a q s t\<close> have "sugg s i ?b q = None" by auto
-    with 3 have "dsa.proved_safe_at (ballot s) (vote s i) q ?b v" by simp 
-    thus ?thesis 
-      using "1" "4" "5" None assms(4) assms(5) dsa_p.proved_safe_at_imp_safe_at safe_at_def by fastforce 
+    with 3 have "dsa.proved_safe_at (ballot s) (flip (vote s) i) q ?b v" by simp 
+    thus ?thesis  using "1" "4" "5" None assms(4) assms(5) dsa_p.proved_safe_at_imp_safe_at 
+      by (simp add: safe_at_def conservative_def dsa_p.proved_safe_at_imp_safe_at)
   next
     case (Some w)
     from Some 6 have 7:"sugg s i ?b q = Some w" by auto
-    hence "dsa.proved_safe_at (ballot s) (vote s i) q ?b w" using "3" by auto 
-    with \<open>safe s\<close> and \<open>conservative_array s\<close> show ?thesis using 6 7 4 5 3 1
-      by (simp add: dsa_p.proved_safe_at_imp_safe_at safe_at_def)
+    hence "dsa.proved_safe_at (ballot s) (flip (vote s) i) q ?b w" using "3" by auto 
+    with \<open>safe s\<close> and \<open>conservative s\<close> show ?thesis using 6 7 4 5 3 1
+      by (simp add: conservative_def dsa_p.proved_safe_at_imp_safe_at safe_at_def)
   qed
 qed
 
@@ -269,46 +269,62 @@ lemma inv5:"invariant the_ioa inv5"
     note mono = \<open>\<And>i v b. safe_at s i v b \<Longrightarrow> safe_at t i v b\<close>
     show "safe t" using \<open>inv5 s\<close> mono and \<open>acquire_leadership a q s t\<close> by (simp add:inv5_def)
     have "safe s" using inv5_def \<open>inv5 s\<close> by blast
-    note aqcuire_leadership_safe[OF \<open>acquire_leadership a q s t\<close> \<open>inv4 s\<close> \<open>safe s\<close> \<open>conservative_array s\<close>]
+    note aqcuire_leadership_safe[OF \<open>acquire_leadership a q s t\<close> \<open>inv4 s\<close> \<open>safe s\<close> \<open>conservative s\<close>]
     moreover have "ballot t = ballot s" and "vote t = vote s" 
       and "\<And> b i . b \<noteq> ballot s a \<Longrightarrow> suggestion t i b = suggestion s i b" 
       and "is_leader t = (is_leader s)(a := True)" using \<open>acquire_leadership a q s t\<close> by simp_all
     ultimately show " \<forall>i b. case suggestion t i b of None \<Rightarrow>
       is_leader t (leader b) \<and> ballot t (leader b) = b \<longrightarrow> (\<forall>v. safe_at t i v b)
       | Some v \<Rightarrow> safe_at t i v b" using mono \<open>inv5 s\<close> \<open>inv1 s\<close> mono
-      apply (simp add:inv5_def inv1_def split:option.splits)
-      by (metis (no_types, lifting) option.case_eq_if option.distinct(1) option.sel)
+      -- {* TODO: make this cleaner. *}
+      apply (auto simp add:inv5_def inv1_def conservative_def split:option.splits)
+         apply (metis option.case_eq_if)
+        apply (metis option.simps(5))
+       apply (metis fun_upd_same inv1_def option.distinct(1) prems(8))
+    proof -
+      fix i :: nat and b :: nat and x2 :: 'b
+      assume a1: "ballot t = ballot s"
+      assume a2: "vote t = vote s"
+      assume a3: "suggestion t i b = Some x2"
+      assume a4: "\<And>b i. b \<noteq> ballot s a \<Longrightarrow> suggestion t i b = suggestion s i b"
+      assume a5: "\<forall>i b. (ballot s (leader b) = b \<longrightarrow> is_leader s (leader b) \<longrightarrow> (\<exists>y. suggestion s i b = Some y) \<or> (\<forall>v. dsa.safe_at (ballot s) (\<lambda>y. vote s y i) v b)) \<and> (\<forall>x2. suggestion s i b = Some x2 \<longrightarrow> dsa.safe_at (ballot s) (\<lambda>y. vote s y i) x2 b)"
+      assume "\<And>i v. case suggestion t i (ballot s a) of None \<Rightarrow> dsa.safe_at (ballot t) (\<lambda>y. vote t y i) v (ballot t a) | Some v \<Rightarrow> dsa.safe_at (ballot t) (\<lambda>y. vote t y i) v (ballot t a)"
+      then have "\<And>n b. case suggestion t n (ballot s a) of None \<Rightarrow> dsa.safe_at (ballot s) (\<lambda>a. vote s a n) b (ballot t a) | Some b \<Rightarrow> dsa.safe_at (ballot t) (\<lambda>a. vote t a n) b (ballot t a)"
+        using a2 a1 by metis
+      then have f6: "\<And>b. case suggestion t i (ballot s a) of None \<Rightarrow> dsa.safe_at (ballot s) (\<lambda>a. vote s a i) b (ballot t a) | Some b \<Rightarrow> dsa.safe_at (ballot t) (\<lambda>a. vote t a i) b (ballot t a)"
+        by blast
+      have f7: "ballot s a = b \<or> suggestion s i b = Some x2"
+        using a4 a3 by (metis (full_types))
+      have "ballot s a = b \<longrightarrow> dsa.safe_at (ballot s) (\<lambda>a. vote s a i) x2 b"
+        using f6 a3 a2 a1 by force
+      then show "dsa.safe_at (ballot s) (\<lambda>a. vote s a i) x2 b"
+        using f7 a5 by blast
+    qed
   qed
   done
 
 definition inv6 where
-  inv6_def[inv_defs]:"inv6 s \<equiv> \<forall> i a b . ballot s a < b \<longrightarrow> vote s i a b = None"
+  inv6_def[inv_defs]:"inv6 s \<equiv> \<forall> i a b . ballot s a < b \<longrightarrow> flip (vote s) i a b = None"
 
 lemma  inv6:"invariant the_ioa inv6"
 by (try_inv)
 
 definition inv7 where inv7_def[inv_defs]:
-  "inv7 s \<equiv> \<forall> i a b v . vote s i a b = Some v \<longrightarrow> safe_at s i v b"
+  "inv7 s \<equiv> \<forall> i a b v . flip (vote s) i a b = Some v \<longrightarrow> safe_at s i v b"
 
 lemma inv7:"invariant the_ioa inv7"
   apply (inv_cases_2 invs:inv5)
         apply (auto simp add:inv7_def ioa_defs inv5_def option.splits) (* automatic from here *)
-  subgoal proof -
-    fix s :: "('b, 'a, ?'l) ampr1_state" and aa :: 'a and i :: nat and v :: 'b
-    assume a1: "vote s i aa (ballot s aa) = None"
-    assume a2: "suggestion s i (ballot s aa) = Some v"
-    assume a3: "\<forall>i a b v. vote s i a b = Some v \<longrightarrow> safe_at s i v b"
-    assume a4: "\<forall>i b. case suggestion s i b of None \<Rightarrow> is_leader s (leader b) \<and> ballot s (leader b) = b \<longrightarrow> (\<forall>v. safe_at s i v b) | Some v \<Rightarrow> safe_at s i v b"
-    assume a5: "\<And>ia va b. safe_at s ia va b \<Longrightarrow> dsa.safe_at (ballot s) (if ia = i then (vote s i)(aa := vote s i aa(ballot s aa \<mapsto> v)) else vote s ia) va b"
-    have "\<And>n na. suggestion s n na = None \<or> safe_at s n (the (suggestion s n na)) na"
-      using a4 by (simp add: option.case_eq_if)
-    then have "safe_at s i v (ballot s aa)"
-      using a3 a2 a1 by (metis option.sel)
-    then show "dsa.safe_at (ballot s) ((vote s i)(aa := vote s i aa(ballot s aa \<mapsto> v))) v (ballot s aa)"
-      using a5 by presburger
-  qed
-   apply presburger
-  by fastforce
+proof -
+  fix s :: "('b, 'a, ?'l) ampr1_state" and aa :: 'a and i :: nat and v :: 'b
+  assume a1: "\<And>ia va b. dsa.safe_at (ballot s) (\<lambda>y. vote s y ia) va b \<Longrightarrow> dsa.safe_at (ballot s) (\<lambda>y. (if y = aa then (vote s aa)(i := vote s aa i(ballot s aa \<mapsto> v)) else vote s y) ia) va b"
+  assume a2: "\<forall>i b. case suggestion s i b of None \<Rightarrow> is_leader s (leader b) \<and> ballot s (leader b) = b \<longrightarrow> (\<forall>v. dsa.safe_at (ballot s) (\<lambda>y. vote s y i) v b) | Some v \<Rightarrow> dsa.safe_at (ballot s) (\<lambda>y. vote s y i) v b"
+  assume "suggestion s i (ballot s aa) = Some v"
+  then have "case Some v of None \<Rightarrow> is_leader s (leader (ballot s aa)) \<and> ballot s (leader (ballot s aa)) = ballot s aa \<longrightarrow> (\<forall>b. dsa.safe_at (ballot s) (\<lambda>a. vote s a i) b (ballot s aa)) | Some b \<Rightarrow> dsa.safe_at (ballot s) (\<lambda>a. vote s a i) b (ballot s aa)"
+    using a2 by metis
+  then show "dsa.safe_at (ballot s) (\<lambda>a. (if a = aa then (vote s aa)(i := vote s aa i(ballot s aa \<mapsto> v)) else vote s a) i) v (ballot s aa)"
+    using a1 by simp
+qed
   
 end
 
